LeanIMP/ImpState.lean
@@ -2,10 +2,10 @@ import LeanIMP.Basic
 
 
 def IMPState.ext_eq (s1 s2 : IMPState) : Prop :=
-  forall (k : String), IMPState.lookup s1 k = IMPState.lookup s2 k
+  forall (k : String), s1.lookup k = s2.lookup k
 
 theorem IMPState.lookup_congr (k : String) {s1 s2 : IMPState} (h : IMPState.ext_eq s1 s2) :
-  IMPState.lookup s1 k = IMPState.lookup s2 k :=
+  s1.lookup k = s2.lookup k :=
   h k
 
 theorem IMPState.ext_eq_reflexive (s : IMPState) : IMPState.ext_eq s s :=
@@ -44,50 +44,31 @@ theorem IMPState.update_twice_eq_update_once (s : IMPState) (k_update : String) 
       intros k
       cases h_lem_bool: k == k_update with
         | true =>
-          unfold lookup
-          simp
+          unfold List.lookup
           unfold update
-          unfold List.find?
           simp
-          cases h_eq_bool : (k_update == k) with
-            | true => simp
-            | false =>
-              have h_lem : k = k_update := by
-                apply decide_eq_true_iff.mp
-                exact h_lem_bool
-              rw [h_lem] at h_eq_bool
-              conv at h_eq_bool =>
-                lhs
-                rw [beq_self_eq_true]
-              contradiction -- contradiction, we are in the case where they are equal
+          rw [h_lem_bool]
         | false =>
-          unfold lookup
-          simp
+          unfold List.lookup
           unfold update
-          unfold List.find?
           simp
-          cases h_eq_bool : (k_update == k) with
-            | true => simp -- contradiction, we are in the case where they are not equal
-            | false =>
+          rw [h_lem_bool]
+          simp
+          unfold List.lookup
+          rw [h_lem_bool]
+          simp
+          match s with
+            | List.nil => simp
+            | List.cons head tail =>
               simp
-              conv =>
-                lhs
-                unfold List.find?
-              simp
-              cases h_eq_bool2 : (k_update == k) with
-              | true =>
-                rw [h_eq_bool2] at h_eq_bool
-                contradiction -- contradiction, we are in the case where they are not equal
-              | false =>
-                simp
+              rw [List.lookup]
 
 
-theorem IMPState.update_unrelated_eq_update_once (s : IMPState) (k1 k2: String) (v1 v2 : Int) (k1_neq_k2 : ¬(k1 = k2)) :
-  (IMPState.update (s.update k1 v1) k2 v2).lookup k1 = (s.update k1 v1).lookup k1 :=
+theorem IMPState.update_unrelated_eq_update_once (s : IMPState) (k1 k2: String) (v2 : Int) (k1_neq_k2 : ¬(k1 = k2)) :
+  (IMPState.update s k2 v2).lookup k1 = s.lookup k1 :=
   by
     unfold update
     unfold List.lookup
-    simp
     cases h_eq_bool : (k1 == k2) with
       | true =>
         have eq : k1 = k2 := by
@@ -95,4 +76,68 @@ theorem IMPState.update_unrelated_eq_update_once (s : IMPState) (k1 k2: String) 
           exact h_eq_bool -- contradiction, we have an assumption that contradicts that
         contradiction
       | false =>
+        match s with
+          | List.nil => simp
+          | List.cons head tail =>
+            simp
+            conv =>
+              lhs
+              unfold List.lookup
+
+
+
+theorem IMPState.prepend_update_eq_reverse_append (s1 s2: IMPState) :
+  s1.prepend_updates s2 = s2.append s1 :=
+  by
+    induction s2 generalizing s1 with
+    | nil =>
+      unfold prepend_updates
+      simp
+    | cons head tail ih =>
+      -- step case
+      unfold prepend_updates
+      simp
+      unfold IMPState.update
+      unfold List.foldr
+      simp
+      match tail with
+        | List.nil => simp
+        | List.cons _ _ =>
+          simp
+
+theorem IMPState.prepend_update_eq_reverse_Happend (s1 s2: IMPState) :
+  s1.prepend_updates s2 = s2 ++ s1 :=
+  by
+    exact IMPState.prepend_update_eq_reverse_append s1 s2
+
+
+theorem IMPState.update_unrelated_eq_update_list (s1 s2 : IMPState) (k: String) (s2_does_not_contain : IMPState.does_not_contain s2 k) :
+  (s1.prepend_updates s2).lookup k = s1.lookup k :=
+  by
+    induction s2 generalizing s1 with
+    | nil =>
+      unfold prepend_updates
+      simp
+    | cons head tail ih =>
+      unfold prepend_updates
+      simp
+      unfold update
+      have head_is_not_prop : Not (head.fst = k) := by
+        apply s2_does_not_contain.left
+      have head_is_not : (head.fst == k) = false := by
+        rw [<- Bool.not_eq_true]
         simp
+        exact head_is_not_prop
+      have head_is_not_symm : (k == head.fst) = false := by
+        conv =>
+          arg 1
+          rw [BEq.comm]
+        exact head_is_not
+      conv =>
+        lhs
+        unfold List.lookup
+      rw [head_is_not_symm]
+      simp
+      rw [<- IMPState.prepend_update_eq_reverse_Happend]
+      apply ih
+      exact s2_does_not_contain.right
